Moved list sort instance to separate file

theories/examples/list_sort.v
@@ -3,9 +3,6 @@ From osiris.channel Require Import proto_channel.
 From iris.heap_lang Require Import proofmode notation.
 From osiris.utils Require Import list.
 
-Definition compare_vals : val :=
-    λ: "x" "y", "x" ≤ "y".
-
 Definition lmerge : val :=
   rec: "go" "cmp" "hys" "hzs" :=
     match: "hys" with
@@ -216,38 +213,4 @@ Section list_sort.
     wp_pures. iApply "HΦ". iFrame.
   Qed.
 
-  (* Example: Sort of integers *)
-  Definition IZ (x : Z) (v : val) : iProp Σ :=
-    ⌜∃ w, v = LitV $ LitInt w ∧ x = w⌝%I.
-
-  Lemma compare_vals_spec : cmp_spec IZ (≤) compare_vals.
-  Proof.
-    iIntros (x x' v v' Φ) "!>".
-    iIntros ([[w [-> ->]] [w' [-> ->]]]) "HΦ".
-    wp_lam. wp_pures. iApply "HΦ". eauto 10 with iFrame.
-  Qed.
-
-  Local Arguments val_encode _ _ !_ /.
-
-  Lemma list_sort_client_le_spec l (xs : list Z) :
-    {{{ l ↦ val_encode xs }}}
-      list_sort_client compare_vals #l
-    {{{ ys, RET #(); ⌜Sorted (≤) ys⌝ ∗ ⌜ ys ≡ₚ xs⌝ ∗ l ↦ val_encode ys }}}.
-  Proof.
-    assert (∀ zs : list Z, val_encode zs = val_encode (LitV ∘ LitInt <$> zs)) as Henc.
-    { intros zs. induction zs; f_equal/=; auto with f_equal. }
-    iIntros (Φ) "Hl HΦ".
-    iApply (list_sort_client_spec IZ (≤) _ _ (LitV ∘ LitInt <$> xs) xs with "[] [Hl] [HΦ]").
-    { iApply compare_vals_spec. }
-    { rewrite -Henc. iFrame "Hl".
-      iInduction xs as [|x xs] "IH"; csimpl; first by iFrame.
-      iFrame "IH". by iExists x. }
-    iIntros "!>" (ys ws) "(?&?&?&HI)".
-    iAssert ⌜ ws = (LitV ∘ LitInt) <$> ys ⌝%I with "[HI]" as %->.
-    { iInduction ys as [|y ys] "IH" forall (ws);
-        destruct ws as [|w ws]; csimpl; try done.
-      iDestruct "HI" as "[HI1 HI2]"; iDestruct "HI1" as %(?&->&->).
-      by iDestruct ("IH" with "HI2") as %->. }
-    rewrite -Henc. iApply ("HΦ" $! ys with "[$]").
-  Qed.
 End list_sort.
