theories/examples/list_sort_instances.v
@@ -1,0 +1,48 @@
+From stdpp Require Import sorting.
+From osiris.channel Require Import proto_channel.
+From iris.heap_lang Require Import proofmode notation.
+From osiris.utils Require Import list.
+From osiris.examples Require Import list_sort.
+
+Section list_sort_instances.
+  Context `{!heapG Σ, !proto_chanG Σ} (N : namespace).
+
+  (* Example: Sort of integers *)
+  Definition IZ (x : Z) (v : val) : iProp Σ :=
+    ⌜∃ w, v = LitV $ LitInt w ∧ x = w⌝%I.
+
+  Definition compareZ : val :=
+    λ: "x" "y", "x" ≤ "y".
+
+  Lemma compareZ_spec : cmp_spec IZ (≤) compareZ.
+  Proof.
+    iIntros (x x' v v' Φ) "!>".
+    iIntros ([[w [-> ->]] [w' [-> ->]]]) "HΦ".
+    wp_lam. wp_pures. iApply "HΦ". eauto 10 with iFrame.
+  Qed.
+  
+  Local Arguments val_encode _ _ !_ /.
+
+  Lemma list_sort_client_le_spec l (xs : list Z) :
+    {{{ l ↦ val_encode xs }}}
+      list_sort_client compareZ #l
+      {{{ ys, RET #(); ⌜Sorted (≤) ys⌝ ∗ ⌜ ys ≡ₚ xs⌝ ∗ l ↦ val_encode ys }}}.
+  Proof.
+    assert (∀ zs : list Z, val_encode zs = val_encode (LitV ∘ LitInt <$> zs)) as Henc.
+    { intros zs. induction zs; f_equal/=; auto with f_equal. }
+    iIntros (Φ) "Hl HΦ".
+    iApply (list_sort_client_spec N IZ (≤) _ _ (LitV ∘ LitInt <$> xs) xs with "[] [Hl] [HΦ]").
+    { iApply compareZ_spec. }
+    { rewrite -Henc. iFrame "Hl".
+      iInduction xs as [|x xs] "IH"; csimpl; first by iFrame.
+      iFrame "IH". by iExists x. }
+    iIntros "!>" (ys ws) "(?&?&?&HI)".
+    iAssert ⌜ ws = (LitV ∘ LitInt) <$> ys ⌝%I with "[HI]" as %->.
+    { iInduction ys as [|y ys] "IH" forall (ws);
+      destruct ws as [|w ws]; csimpl; try done.
+      iDestruct "HI" as "[HI1 HI2]"; iDestruct "HI1" as %(?&->&->).
+      by iDestruct ("IH" with "HI2") as %->. }
+    rewrite -Henc. iApply ("HΦ" $! ys with "[$]").
+  Qed.
+
+End list_sort_instances.
